some more tests

Impl/BookkeepingModel.i.dfy
@@ -305,6 +305,82 @@ module BookkeepingModel {
     )
   }
 
+  predicate writeWithNode(s: ImplVariables, ref: BT.G.Reference, node: Node, s': ImplVariables)
+  requires s.W()
+  requires s.WriteAllocConditions()
+  requires s.ChildrenConditions(node.children)
+  requires s.cache.Inv()
+  {
+    var children := node.children;
+    var succs := if children.Some? then children.value else [];
+    var oldLoc := MapLookupOption(s.ephemeralIndirectionTable.locs, ref);
+    lemmaIndirectionTableLocIndexValid(s, ref);
+    var blockAllocator' := if oldLoc.Some?
+      then BlockAllocatorModel.MarkFreeEphemeral(s.blockAllocator.I(), oldLoc.value.addr as int / NodeBlockSize())
+      else s.blockAllocator.I();
+    var eph := s.ephemeralIndirectionTable.I().
+      (graph := s.ephemeralIndirectionTable.graph[ref := succs]).
+      (locs := MapRemove1(s.ephemeralIndirectionTable.locs, ref)).
+      (refUpperBound := if ref > s.ephemeralIndirectionTable.refUpperBound then ref else s.ephemeralIndirectionTable.refUpperBound);
+
+    && s'.Ready?
+    && s'.blockAllocator.Inv()
+    && s'.cache.Inv()
+
+    && s'.ephemeralIndirectionTable.I() == eph
+    && s'.lru.Queue() == LruModel.Use(s.lru.Queue(), ref)
+    && s'.blockAllocator.I() == blockAllocator'
+    && s'.persistentIndirectionTable == s.persistentIndirectionTable
+    && s'.frozenIndirectionTable == s.frozenIndirectionTable
+    && s'.persistentIndirectionTableLoc == s.persistentIndirectionTableLoc
+    && s'.frozenIndirectionTableLoc == s.frozenIndirectionTableLoc
+    && s'.outstandingIndirectionTableWrite == s.outstandingIndirectionTableWrite
+    && s'.outstandingBlockWrites == s.outstandingBlockWrites
+    && s'.outstandingBlockReads == s.outstandingBlockReads
+    && s'.cache.I() == s.cache.I()[ref := node]
+  }
+
+  // lemma writeBookkeepingBitmapCorrect(s: ImplVariables, ref: BT.G.Reference, children: Option<seq<BT.G.Reference>>)
+  // requires WriteAllocConditions(s)
+  // requires ChildrenConditions(s, children)
+  // requires |s.ephemeralIndirectionTable.graph| < IT.MaxSize()
+  // ensures var s' := writeBookkeeping(s, ref, children);
+  //   && WriteAllocConditions(s')
+  // {
+  // }
+
+  lemma writeCorrect(s: ImplVariables, ref: BT.G.Reference, node: Node, s': ImplVariables)
+  requires s.Ready?
+  requires s.WFBCVars()
+  requires s.WriteAllocConditions()
+  requires ref in s.ephemeralIndirectionTable.I().graph
+  requires ref in s.cache.I()
+  requires WFNode(node)
+  requires BC.BlockPointsToValidReferences(node, s.ephemeralIndirectionTable.graph)
+  requires s.frozenIndirectionTable.lSome? && ref in s.frozenIndirectionTable.value.graph ==> ref in s.frozenIndirectionTable.value.locs
+  requires |s.ephemeralIndirectionTable.graph| < IT.MaxSize()
+  requires writeWithNode(s, ref, node, s')
+
+  // ensures s'.WFBCVars()
+    // && BC.Dirty(IBlockCache(s), IBlockCache(s'), ref, INode(node))
+    // && TotalCacheSize(s') == TotalCacheSize(s)
+    // && WriteAllocConditions(s')
+  {
+    lemmaIndirectionTableLocIndexValid(s, ref);
+    WeightBucketEmpty();
+
+    LruModel.LruUse(s.lru.Queue(), ref);
+
+    assert s'.W();
+
+    // writeBookkeepingBitmapCorrect(s, ref, node.children);
+    // reveal_writeBookkeeping();
+
+    // var s' := writeWithNode(s, ref, node);
+    // assert WFBCVars(s');
+  }
+
+
 
 /*
   // Conditions that will hold intermediately between writes and allocs
@@ -368,32 +444,6 @@ module BookkeepingModel {
   // because it turns out to be easier to do the cache updates separately. However, for the proofs
   // it is easier to use the below.
 
-  function writeWithNode(s: ImplVariables, ref: BT.G.Reference, node: Node)
-  : (s': ImplVariables)
-  requires WriteAllocConditions(s)
-  requires ChildrenConditions(s, node.children)
-  requires |s.ephemeralIndirectionTable.graph| < IT.MaxSize()
-  ensures WriteAllocConditions(s')
-  ensures |s'.ephemeralIndirectionTable.graph| <= |s.ephemeralIndirectionTable.graph| + 1
-  {
-    lemmaIndirectionTableLocIndexValid(s, ref);
-    var (eph, oldLoc) := s.ephemeralIndirectionTable.updateAndRemoveLoc(ref,
-        (if node.children.Some? then node.children.value else []));
-    var blockAllocator' := if oldLoc.Some?
-      then BlockAllocatorModel.MarkFreeEphemeral(s.blockAllocator, oldLoc.value.addr as int / NodeBlockSize())
-      else s.blockAllocator;
-    var s' := s.(ephemeralIndirectionTable := eph).(cache := s.cache[ref := node])
-        .(lru := LruModel.Use(s.lru, ref))
-        .(blockAllocator := blockAllocator');
-
-    freeIndirectionTableLocCorrect(s, s', ref,
-      if oldLoc.Some?
-      then Some(oldLoc.value.addr as int / NodeBlockSize())
-      else None);
-    reveal_ConsistentBitmap();
-
-    s'
-  }
 
   function allocWithNode(s: ImplVariables, node: Node)
   : (p: (ImplVariables, Option<Reference>))
@@ -412,167 +462,7 @@ module BookkeepingModel {
     )
   }
 
-  lemma freeIndirectionTableLocCorrect(
-      s: ImplVariables, s': ImplVariables, ref: BT.G.Reference, j: Option<int>)
-  requires WriteAllocConditions(s)
-  requires s'.Ready?
-  requires forall r | r != ref ::
-      MapsAgreeOnKey(
-          s.ephemeralIndirectionTable.I().locs,
-          s'.ephemeralIndirectionTable.I().locs,
-          r)
-  requires ref !in s'.ephemeralIndirectionTable.I().locs
-  requires j.Some? ==> 0 <= j.value < NumBlocks()
-  requires j.Some? ==> ref in s.ephemeralIndirectionTable.I().locs
-  requires j.Some? ==> s.ephemeralIndirectionTable.I().locs[ref].addr as int == j.value * NodeBlockSize()
-  requires j.Some? ==> s'.blockAllocator == BlockAllocatorModel.MarkFreeEphemeral(s.blockAllocator, j.value)
-  requires j.None? ==> s'.blockAllocator == s.blockAllocator
-  requires j.None? ==> ref !in s.ephemeralIndirectionTable.I().locs
-  ensures (forall i: int :: IT.IndirectionTable.IsLocAllocIndirectionTable(s'.ephemeralIndirectionTable.I(), i)
-      <==> IT.IndirectionTable.IsLocAllocBitmap(s'.blockAllocator.ephemeral, i))
-  ensures BlockAllocatorModel.Inv(s'.blockAllocator)
-  ensures BC.AllLocationsForDifferentRefsDontOverlap(
-        s'.ephemeralIndirectionTable.I())
-  ensures (forall loc |
-        loc in s'.ephemeralIndirectionTable.I().locs.Values :: 
-          DiskLayout.ValidNodeLocation(loc))
-  {
-    reveal_ConsistentBitmap();
-    BitmapModel.reveal_IsSet();
-    BitmapModel.reveal_BitUnset();
-    lemmaIndirectionTableLocIndexValid(s, ref);
 
-    forall r1, r2 | r1 in s'.ephemeralIndirectionTable.I().locs && r2 in s'.ephemeralIndirectionTable.I().locs
-    ensures BC.LocationsForDifferentRefsDontOverlap(s'.ephemeralIndirectionTable.I(), r1, r2)
-    {
-      assert MapsAgreeOnKey( s.ephemeralIndirectionTable.I().locs, s'.ephemeralIndirectionTable.I().locs, r1);
-      assert MapsAgreeOnKey( s.ephemeralIndirectionTable.I().locs, s'.ephemeralIndirectionTable.I().locs, r2);
-    }
-
-    forall loc | loc in s'.ephemeralIndirectionTable.I().locs.Values
-    ensures DiskLayout.ValidNodeLocation(loc)
-    {
-      var r :| r in s'.ephemeralIndirectionTable.I().locs && s'.ephemeralIndirectionTable.I().locs[r] == loc;
-      assert MapsAgreeOnKey(s.ephemeralIndirectionTable.I().locs, s'.ephemeralIndirectionTable.I().locs, r);
-    }
-
-    if j.Some? {
-      assert DiskLayout.ValidNodeLocation(s.ephemeralIndirectionTable.I().locs[ref]);
-      assert j.value >= MinNodeBlockIndex() by {
-        DiskLayout.reveal_ValidNodeAddr();
-      }
-    }
-
-    forall i: int
-    | IT.IndirectionTable.IsLocAllocIndirectionTable(s'.ephemeralIndirectionTable.I(), i)
-    ensures IT.IndirectionTable.IsLocAllocBitmap(s'.blockAllocator.ephemeral, i)
-    {
-      if j.Some? && i == j.value {
-        if 0 <= i < MinNodeBlockIndex() {
-          assert false;
-        } else {
-          var r :| r in s'.ephemeralIndirectionTable.locs &&
-              s'.ephemeralIndirectionTable.locs[r].addr as int == i * NodeBlockSize() as int;
-          assert MapsAgreeOnKey(
-            s.ephemeralIndirectionTable.I().locs,
-            s'.ephemeralIndirectionTable.I().locs, r);
-
-          assert BC.LocationsForDifferentRefsDontOverlap(s.ephemeralIndirectionTable.I(), ref, r);
-
-          assert ref !in s'.ephemeralIndirectionTable.I().locs;
-          assert r in s'.ephemeralIndirectionTable.I().locs;
-          assert s.ephemeralIndirectionTable.I().locs[r]
-              == s.ephemeralIndirectionTable.I().locs[ref];
-          assert r == ref;
-
-          assert false;
-        }
-      } else {
-        if 0 <= i < MinNodeBlockIndex() {
-          assert IT.IndirectionTable.IsLocAllocIndirectionTable(s.ephemeralIndirectionTable.I(), i);
-          assert IT.IndirectionTable.IsLocAllocBitmap(s.blockAllocator.ephemeral, i);
-          assert IT.IndirectionTable.IsLocAllocBitmap(s'.blockAllocator.ephemeral, i);
-        } else {
-          var r :| r in s'.ephemeralIndirectionTable.locs &&
-              s'.ephemeralIndirectionTable.locs[r].addr as int == i * NodeBlockSize() as int;
-          assert MapsAgreeOnKey(
-            s.ephemeralIndirectionTable.I().locs,
-            s'.ephemeralIndirectionTable.I().locs, r);
-          assert IT.IndirectionTable.IsLocAllocIndirectionTable(s.ephemeralIndirectionTable.I(), i);
-          assert IT.IndirectionTable.IsLocAllocBitmap(s.blockAllocator.ephemeral, i);
-          assert IT.IndirectionTable.IsLocAllocBitmap(s'.blockAllocator.ephemeral, i);
-        }
-      }
-    }
-
-    forall i: int
-    | IT.IndirectionTable.IsLocAllocBitmap(s'.blockAllocator.ephemeral, i)
-    ensures IT.IndirectionTable.IsLocAllocIndirectionTable(s'.ephemeralIndirectionTable.I(), i)
-    {
-      if j.Some? && i == j.value {
-        assert IT.IndirectionTable.IsLocAllocIndirectionTable(s'.ephemeralIndirectionTable.I(), i);
-      } else {
-        assert IT.IndirectionTable.IsLocAllocBitmap(s.blockAllocator.ephemeral, i);
-        assert IT.IndirectionTable.IsLocAllocIndirectionTable(s.ephemeralIndirectionTable.I(), i);
-        if 0 <= i < MinNodeBlockIndex() {
-          assert IT.IndirectionTable.IsLocAllocIndirectionTable(s'.ephemeralIndirectionTable.I(), i);
-        } else {
-          var r :| r in s.ephemeralIndirectionTable.locs &&
-            s.ephemeralIndirectionTable.locs[r].addr as int == i * NodeBlockSize() as int;
-          assert MapsAgreeOnKey(
-            s.ephemeralIndirectionTable.I().locs,
-            s'.ephemeralIndirectionTable.I().locs, r);
-          assert r in s'.ephemeralIndirectionTable.locs &&
-            s'.ephemeralIndirectionTable.locs[r].addr as int == i * NodeBlockSize() as int;
-          assert IT.IndirectionTable.IsLocAllocIndirectionTable(s'.ephemeralIndirectionTable.I(), i);
-        }
-      }
-    }
-
-    if j.Some? {
-      forall i | 0 <= i < NumBlocks()
-      ensures BitmapModel.IsSet(s'.blockAllocator.full, i) == (
-        || BitmapModel.IsSet(s'.blockAllocator.ephemeral, i)
-        || (s'.blockAllocator.frozen.Some? && BitmapModel.IsSet(s'.blockAllocator.frozen.value, i))
-        || BitmapModel.IsSet(s'.blockAllocator.persistent, i)
-        || BitmapModel.IsSet(s'.blockAllocator.full, i)
-      )
-      {
-        if i == j.value {
-        } else {
-          assert BitmapModel.IsSet(s'.blockAllocator.full, i) == BitmapModel.IsSet(s.blockAllocator.full, i);
-          assert BitmapModel.IsSet(s'.blockAllocator.ephemeral, i) == BitmapModel.IsSet(s.blockAllocator.ephemeral, i);
-          assert s'.blockAllocator.frozen.Some? ==> BitmapModel.IsSet(s'.blockAllocator.frozen.value, i) == BitmapModel.IsSet(s.blockAllocator.frozen.value, i);
-          assert BitmapModel.IsSet(s'.blockAllocator.persistent, i) == BitmapModel.IsSet(s.blockAllocator.persistent, i);
-          assert BitmapModel.IsSet(s'.blockAllocator.outstanding, i) == BitmapModel.IsSet(s.blockAllocator.outstanding, i);
-        }
-      }
-    } else {
-    }
-  }
-
-  lemma writeBookkeepingBitmapCorrect(s: ImplVariables, ref: BT.G.Reference, children: Option<seq<BT.G.Reference>>)
-  requires WriteAllocConditions(s)
-  requires ChildrenConditions(s, children)
-  requires |s.ephemeralIndirectionTable.graph| < IT.MaxSize()
-  ensures var s' := writeBookkeeping(s, ref, children);
-    && WriteAllocConditions(s')
-  {
-    /*reveal_writeBookkeeping();
-    var s' := writeBookkeeping(s, ref, children);
-
-    lemmaIndirectionTableLocIndexValid(s, ref);
-    assert s.ephemeralIndirectionTable.count as nat < 0x10000000000000000 / 8;
-    var (eph, oldEntry) := MutableMapModel.InsertAndGetOld(s.ephemeralIndirectionTable, ref,
-        (None, if children.Some? then children.value else []));
-
-    var j := if oldEntry.Some? && oldEntry.value.0.Some? then
-      Some(oldEntry.value.0.value.addr as int / NodeBlockSize())
-    else
-      None;
-    freeIndirectionTableLocCorrect(s, s', ref, j);
-    reveal_ConsistentBitmap();*/
-  }
 
   lemma allocCorrect(s: ImplVariables, node: Node)
   requires WFBCVars(s)
@@ -839,400 +729,4 @@ module BookkeepingModel {
     reveal_writeBookkeeping();
   }
 */
-
-/*
-  predicate ChildrenConditions(s: BBC.Variables, succs: Option<seq<BT.G.Reference>>)
-  requires s.Ready?
-  {
-    succs.Some? ==> (
-      && |succs.value| <= MaxNumChildren()
-      && IT.IndirectionTable.SuccsValid(succs.value, s.ephemeralIndirectionTable.graph)
-    )
-  }
-
-  lemma lemmaIndirectionTableLocIndexValid(s: BBC.Variables, ref: BT.G.Reference)
-  requires s.WriteAllocConditions()
-  ensures ref in s.ephemeralIndirectionTable.locs ==>
-    (
-      // && 0 <= s.ephemeralIndirectionTable.locs[ref].addr as int / NodeBlockSize() < NumBlocks()
-      && (s.ephemeralIndirectionTable.locs[ref].addr as int / NodeBlockSize()) * NodeBlockSize() == s.ephemeralIndirectionTable.locs[ref].addr as int
-    )
-  {
-    if ref in s.ephemeralIndirectionTable.locs {
-      var loc := s.ephemeralIndirectionTable.locs[ref];
-      var i := loc.addr as int / NodeBlockSize();
-      assert s.ephemeralIndirectionTable.locs[ref] == loc;
-      assert loc in s.ephemeralIndirectionTable.locs.Values;
-      assert DiskLayout.ValidNodeLocation(loc);
-      DiskLayout.reveal_ValidNodeAddr();
-      assert i * NodeBlockSize() == loc.addr as int;
-    }
-  }
-
-  // Bookkeeping only - we update the cache with the Node separately.
-  // This turns out to be easier to do.
-
-  function {:opaque} writeBookkeeping(s: BBC.Variables, ref: BT.G.Reference, children: Option<seq<BT.G.Reference>>)
-  : (s': BBC.Variables)
-  requires s.WriteAllocConditions()
-  requires ChildrenConditions(s, children)
-  // requires |s.ephemeralIndirectionTable.graph| < IT.MaxSize()
-  ensures s'.Ready?
-  ensures s'.cache == s.cache
-  ensures s'.WriteAllocConditions()
-  ensures |s'.ephemeralIndirectionTable.graph| <= |s.ephemeralIndirectionTable.graph| + 1
-  {
-    // lemmaIndirectionTableLocIndexValid(s, ref);
-    var succs := if children.Some? then children.value else [];
-    // var oldLoc := MapLookupOption(s.ephemeralIndirectionTable.locs, ref);
-    // TODO(andreal) s.ephemeralIndirectionTable.updateAndRemoveLoc(ref,
-    // TODO(andreal)     (if children.Some? then children.value else []));
-    var eph := s.ephemeralIndirectionTable.(
-      graph := s.ephemeralIndirectionTable.graph[ref := succs]).
-      (locs := MapRemove1(s.ephemeralIndirectionTable.locs, ref)).
-      (refUpperBound := if ref > s.ephemeralIndirectionTable.refUpperBound then ref else s.ephemeralIndirectionTable.refUpperBound);
-
-    var s' := s.(ephemeralIndirectionTable := eph);
-    s'
-  }
-
-  function {:opaque} allocBookkeeping(s: BBC.Variables, children: Option<seq<BT.G.Reference>>)
-  : (p: (BBC.Variables, Option<BT.G.Reference>))
-  requires s.WriteAllocConditions()
-  requires ChildrenConditions(s, children)
-
-  ensures var (s', id) := p;
-    && s'.Ready?
-    && s'.WriteAllocConditions()
-    && |s'.ephemeralIndirectionTable.graph| <= |s.ephemeralIndirectionTable.graph| + 1
-  {
-    var ref := getFreeRef(s);
-    // var ref: Option<BT.G.Reference> :| ref.Some? ==> RefAvailable(s, ref.value);
-    if ref.Some? then (
-      (writeBookkeeping(s, ref.value, children), ref)
-    ) else (
-      (s, None)
-    )
-  }
-
-  function {:opaque} writeBookkeepingNoSuccsUpdate(s: BBC.Variables, ref: BT.G.Reference)
-  : (s': BBC.Variables)
-  requires s.WriteAllocConditions()
-  requires ref in s.ephemeralIndirectionTable.graph
-  ensures s'.Ready?
-  ensures s'.cache == s.cache
-  ensures s'.WriteAllocConditions()
-  ensures |s'.ephemeralIndirectionTable.graph| <= |s.ephemeralIndirectionTable.graph| + 1
-  {
-    var eph := s.ephemeralIndirectionTable.
-      (locs := MapRemove1(s.ephemeralIndirectionTable.locs, ref));
-
-    var s' := s.(ephemeralIndirectionTable := eph);
-    assert s'.WriteAllocConditions();
-    s'
-  }
-
-  // fullWrite and fullAlloc are like writeBookkeeping/allocBookkeeping, except that fullWrite and fullAlloc update
-  // the cache with the node. In the implementation of betree operations we use the above,
-  // because it turns out to be easier to do the cache updates separately. However, for the proofs
-  // it is easier to use the below.
-
-  function writeWithNode(s: BBC.Variables, ref: BT.G.Reference, node: Node)
-  : (s': BBC.Variables)
-  requires s.WriteAllocConditions()
-  requires ChildrenConditions(s, node.children)
-  // requires |s.ephemeralIndirectionTable.graph| < IT.MaxSize()
-  ensures s'.WriteAllocConditions()
-  ensures |s'.ephemeralIndirectionTable.graph| <= |s.ephemeralIndirectionTable.graph| + 1
-  {
-    // lemmaIndirectionTableLocIndexValid(s, ref);
-    var succs := if node.children.Some? then node.children.value else [];
-    // var oldLoc := MapLookupOption(s.ephemeralIndirectionTable.locs, ref);
-    // var (eph, oldLoc) := s.ephemeralIndirectionTable.updateAndRemoveLoc(ref,
-    //     (if node.children.Some? then node.children.value else []));
-    var table := s.ephemeralIndirectionTable;
-
-    var eph := table.
-      (graph := table.graph[ref := succs]).
-      (locs := MapRemove1(table.locs, ref)).
-      (refUpperBound := if ref > table.refUpperBound then ref else table.refUpperBound);
-
-    var s' := s.(ephemeralIndirectionTable := eph).(cache := s.cache[ref := node]);
-
-    assert s'.WriteAllocConditions();
-    s'
-  }
-
-  function allocWithNode(s: BBC.Variables, node: Node)
-  : (p: (BBC.Variables, Option<BT.G.Reference>))
-  requires s.WriteAllocConditions()
-  requires ChildrenConditions(s, node.children)
-  ensures var (s', id) := p;
-      && s'.WriteAllocConditions()
-      && |s'.ephemeralIndirectionTable.graph| <= |s.ephemeralIndirectionTable.graph| + 1
-  {
-    var ref := getFreeRef(s);
-    if ref.Some? then (
-      (writeWithNode(s, ref.value, node), ref)
-    ) else (
-      (s, None)
-    )
-  }
-
-  lemma writeBookkeepingBitmapCorrect(s: BBC.Variables, ref: BT.G.Reference, children: Option<seq<BT.G.Reference>>)
-  requires s.WriteAllocConditions()
-  requires ChildrenConditions(s, children)
-  ensures var s' := writeBookkeeping(s, ref, children);
-    && s'.WriteAllocConditions()
-  {
-  }
-
-  lemma allocCorrect(s: BBC.Variables, node: Node)
-  requires BBC.Inv(s)
-  requires s.WriteAllocConditions()
-  requires BC.BlockPointsToValidReferences(node, s.ephemeralIndirectionTable.graph)
-  // requires TotalCacheSize(s) <= MaxCacheSize() - 1
-  requires WFNode(node)
-  ensures var (s', ref) := allocWithNode(s, node);
-    && BBC.Inv(s')
-    // && WFBCVars(s')
-    && (ref.Some? ==> BC.Alloc(s, s', ref.value, node))
-    && (ref.None? ==> s' == s)
-    && (ref.Some? ==> s'.totalCacheSize() == s.totalCacheSize() + 1)
-    && s'.WriteAllocConditions()
-  {
-    var ref := getFreeRef(s);
-    if ref.Some? {
-      lemmaIndirectionTableLocIndexValid(s, ref.value);
-      // LruModel.LruUse(s.lru, ref.value);
-      // writeBookkeepingBitmapCorrect(s, ref.value, node.children);
-      reveal_writeBookkeeping();
-
-      // var s' := writeWithNode(s, ref.value, node);
-    }
-  }
-
-  lemma writeCorrect(s: BBC.Variables, ref: BT.G.Reference, node: Node)
-  requires s.Ready?
-  requires BBC.Inv(s)
-  requires s.WriteAllocConditions()
-  requires ref in s.ephemeralIndirectionTable.graph
-  requires ref in s.cache
-  requires WFNode(node)
-  requires BC.BlockPointsToValidReferences(node, s.ephemeralIndirectionTable.graph)
-  requires s.frozenIndirectionTable.Some? && ref in s.frozenIndirectionTable.value.graph ==> ref in s.frozenIndirectionTable.value.locs
-  // requires |s.ephemeralIndirectionTable.graph| < IT.MaxSize()
-  ensures var s' := writeWithNode(s, ref, node);
-    && BBC.Inv(s')
-    && BC.Dirty(s, s', ref, node)
-    && s'.totalCacheSize() == s.totalCacheSize()
-    && s'.WriteAllocConditions()
-  {
-    // lemmaIndirectionTableLocIndexValid(s, ref);
-    WeightBucketEmpty();
-    reveal_writeBookkeeping();
-  }
- 
-  lemma writeNewRefIsAlloc(s: BBC.Variables, ref: BT.G.Reference, node: Node)
-  requires s.Ready?
-  requires s.WriteAllocConditions()
-  requires RefAvailable(s, ref)
-  requires WFNode(node)
-  requires BC.WFIndirectionTable(s.ephemeralIndirectionTable)
-  requires BC.BlockPointsToValidReferences(node, s.ephemeralIndirectionTable.graph)
-  ensures var s' := writeWithNode(s, ref, node);
-    && BC.Alloc(s, s', ref, node)
-    && s'.totalCacheSize() == s.totalCacheSize() + 1
-    && s'.WriteAllocConditions()
-  {
-    writeBookkeepingBitmapCorrect(s, ref, node.children);
-  }
-
-  lemma lemmaChildInGraph(s: BBC.Variables, ref: BT.G.Reference, childref: BT.G.Reference)
-  requires s.Ready?
-  requires BBC.Inv(s)
-  requires ref in s.cache
-  requires ref in s.ephemeralIndirectionTable.graph
-  requires childref in BT.G.Successors(s.cache[ref])
-  ensures childref in s.ephemeralIndirectionTable.graph
-  {
-    assert childref in s.ephemeralIndirectionTable.graph[ref];
-  }
-
-  lemma lemmaBlockPointsToValidReferences(s: BBC.Variables, ref: BT.G.Reference)
-  requires BBC.Inv(s)
-  requires s.Ready?
-  requires ref in s.cache
-  requires ref in s.ephemeralIndirectionTable.graph
-  ensures BC.BlockPointsToValidReferences(s.cache[ref], s.ephemeralIndirectionTable.graph);
-  {
-    var node := s.cache[ref];
-    var graph := s.ephemeralIndirectionTable.graph;
-    forall r | r in BT.G.Successors(node) ensures r in graph
-    {
-      lemmaChildInGraph(s, ref, r);
-    }
-  }
-
-  lemma getFreeRefIterateDoesntEqual(s: BBC.Variables, i: uint64, ref: BT.G.Reference)
-  requires s.Ready?
-  requires ref in s.cache
-  requires i >= 1
-  // requires s.ephemeralIndirectionTable.Inv()
-  requires forall r | r in s.ephemeralIndirectionTable.graph :: r < i
-  decreases 0x1_0000_0000_0000_0000 - i as int
-  ensures getFreeRefIterate(s, i) != Some(ref)
-  {
-    if i !in s.cache {
-    } else if i == 0xffff_ffff_ffff_ffff {
-    } else {
-      getFreeRefIterateDoesntEqual(s, i+1, ref);
-    }
-  }
-
-  lemma getFreeRefDoesntEqual(s: BBC.Variables, ref: BT.G.Reference)
-  requires s.Ready?
-  requires ref in s.cache
-  // requires s.ephemeralIndirectionTable.Inv()
-  requires BC.WFIndirectionTable(s.ephemeralIndirectionTable)
-  ensures getFreeRef(s) != Some(ref)
-  {
-    reveal_getFreeRef();
-    var i := s.ephemeralIndirectionTable.refUpperBound;
-    if i == 0xffff_ffff_ffff_ffff {
-    } else {
-      getFreeRefIterateDoesntEqual(s, i+1, ref);
-    }
-  }
-
-  lemma getFreeRef2IterateDoesntEqual(s: BBC.Variables, avoid: BT.G.Reference, i: uint64, ref: BT.G.Reference)
-  requires s.Ready?
-  requires ref in s.cache
-  requires i >= 1
-  requires forall r | r in s.ephemeralIndirectionTable.graph :: r < i
-  ensures getFreeRef2Iterate(s, avoid, i) != Some(ref)
-  decreases 0x1_0000_0000_0000_0000 - i as int
-  {
-    if i != avoid && i !in s.cache {
-    } else if i == 0xffff_ffff_ffff_ffff {
-    } else {
-      getFreeRef2IterateDoesntEqual(s, avoid, i+1, ref);
-    }
-  }
-
-  lemma getFreeRef2DoesntEqual(s: BBC.Variables, avoid: BT.G.Reference, ref: BT.G.Reference)
-  requires s.Ready?
-  requires ref in s.cache
-  requires BC.WFIndirectionTable(s.ephemeralIndirectionTable)
-  ensures getFreeRef2(s, avoid) != Some(ref)
-  {
-    reveal_getFreeRef2();
-    var i := s.ephemeralIndirectionTable.refUpperBound;
-    if i == 0xffff_ffff_ffff_ffff {
-    } else {
-      getFreeRef2IterateDoesntEqual(s, avoid, i+1, ref);
-    }
-  }
-
-  lemma allocRefDoesntEqual(s: BBC.Variables, children: Option<seq<BT.G.Reference>>, ref: BT.G.Reference)
-  requires allocBookkeeping.requires(s, children);
-  requires ref in s.cache
-  requires BC.WFIndirectionTable(s.ephemeralIndirectionTable)
-  ensures allocBookkeeping(s, children).1 != Some(ref)
-  {
-    reveal_allocBookkeeping();
-    getFreeRefDoesntEqual(s, ref);
-  }
-
-  lemma lemmaChildrenConditionsOfNode(
-      s: BBC.Variables, ref: BT.G.Reference)
-  requires s.Ready?
-  requires BBC.Inv(s)
-  requires ref in s.cache
-  requires ref in s.ephemeralIndirectionTable.graph
-  ensures ChildrenConditions(s, s.cache[ref].children)
-  {
-    if s.cache[ref].children.Some? {
-      forall r | r in s.cache[ref].children.value
-      ensures r in s.ephemeralIndirectionTable.graph
-      {
-        // Trigger the forall in CacheConsistentWithSuccessors
-        assert r in BT.G.Successors(s.cache[ref]);
-        assert r in s.ephemeralIndirectionTable.graph[ref];
-      }
-    }
-  }
-
-  lemma lemmaChildrenConditionsSingleOfAllocBookkeeping(
-      s: BBC.Variables, children: Option<seq<BT.G.Reference>>)
-  requires s.WriteAllocConditions()
-  requires ChildrenConditions(s, children)
-  ensures var (s1, newref) := allocBookkeeping(s, children);
-    newref.Some? ==> ChildrenConditions(s1, Some([newref.value]))
-  {
-    reveal_allocBookkeeping();
-    reveal_writeBookkeeping();
-    //assert newref.value in s1.ephemeralIndirectionTable.graph;
-  }
-
-  lemma lemmaChildrenConditionsUpdateOfAllocBookkeeping(
-      s: BBC.Variables, children: Option<seq<BT.G.Reference>>,
-          children1: seq<BT.G.Reference>, i: int)
-  requires s.WriteAllocConditions()
-  requires ChildrenConditions(s, children)
-  requires ChildrenConditions(s, Some(children1))
-  requires 0 <= i < |children1|
-  ensures var (s1, newref) := allocBookkeeping(s, children);
-    newref.Some? ==> ChildrenConditions(s1, Some(children1[i := newref.value]))
-  {
-    reveal_allocBookkeeping();
-    reveal_writeBookkeeping();
-  }
-
-  lemma lemmaChildrenConditionsPreservedWriteBookkeeping(
-      s: BBC.Variables, ref: BT.G.Reference, children: Option<seq<BT.G.Reference>>,
-      children1: Option<seq<BT.G.Reference>>)
-  requires s.WriteAllocConditions()
-  requires ChildrenConditions(s, children)
-  requires ChildrenConditions(s, children1)
-  ensures var s1 := writeBookkeeping(s, ref, children);
-    ChildrenConditions(s1, children1)
-  {
-    reveal_writeBookkeeping();
-  }
-
-  lemma lemmaChildrenConditionsOfReplace1With2(
-      s: BBC.Variables,
-      children: seq<BT.G.Reference>,
-      i: int, a: BT.G.Reference, b: BT.G.Reference)
-  requires s.Ready?
-  requires ChildrenConditions(s, Some(children))
-  requires a in s.ephemeralIndirectionTable.graph
-  requires b in s.ephemeralIndirectionTable.graph
-  requires 0 <= i < |children|
-  requires |children| < MaxNumChildren()
-  ensures ChildrenConditions(s, Some(replace1with2(children, a, b, i)))
-  {
-    reveal_replace1with2();
-  }
-
-  lemma lemmaRefInGraphOfWriteBookkeeping(s: BBC.Variables, ref: BT.G.Reference, children: Option<seq<BT.G.Reference>>)
-  requires s.WriteAllocConditions()
-  requires ChildrenConditions(s, children)
-  ensures var s1 := writeBookkeeping(s, ref, children);
-    ref in s1.ephemeralIndirectionTable.graph
-  {
-    reveal_writeBookkeeping();
-  }
-
-  lemma lemmaRefInGraphPreservedWriteBookkeeping(s: BBC.Variables, ref: BT.G.Reference, children: Option<seq<BT.G.Reference>>, ref2: BT.G.Reference)
-  requires s.WriteAllocConditions()
-  requires ChildrenConditions(s, children)
-  requires ref2 in s.ephemeralIndirectionTable.graph
-  ensures var s1 := writeBookkeeping(s, ref, children);
-    ref2 in s1.ephemeralIndirectionTable.graph
-  {
-    reveal_writeBookkeeping();
-  }
-  */
 }
